Adding halfway through parser

src/cml_utils/Parser.v
@@ -1,18 +1,400 @@
-Require Import String Ascii.
+Require Import String Ascii List Nat Bool.
+Require Import EqClass.
+
+Open Scope string_scope.
+
+(* TODO: Add CharExtra! *)
+Module CharExtra.
+  Definition isDigit : ascii -> bool. Admitted.
+
+  Definition isOctal : ascii -> bool. Admitted.
+
+  Definition isHex : ascii -> bool. Admitted.
+
+  Definition isLower : ascii -> bool. Admitted.
+
+  Definition isUpper : ascii -> bool. Admitted.
+
+  Definition isAlpha : ascii -> bool. Admitted.
+
+  Definition isAlphaNum : ascii -> bool. Admitted.
+
+  Definition isSpace : ascii -> bool. Admitted.
+
+End CharExtra.
 
 Inductive res (A B : Type) :=
 | Ok : A -> res A B
 | Err : B -> res A B.
+Arguments Ok {A} {B}.
+Arguments Err {A} {B}.
 
 Definition nat_to_string : nat -> string. Admitted.
 
-Module Type Parser.
-  Definition stream (A : Type) : Type := (list A * nat * nat).
-  Definition parser (A B : Type) : Type := (stream B) -> ((res A string) * list B * nat * nat).
+Definition cml_unit : Type. Admitted.
+Definition unit_val : cml_unit. Admitted.
 
-  Definition parse {A : Type} (p : (parser A ascii)) (str : string) : (res A string) :=
+Global Instance eqclass_ascii : EqClass ascii := {
+  eqb := Ascii.eqb;
+  eqb_leibniz := Ascii.eqb_eq
+}.
+
+Global Instance eqclass_string : EqClass string := {
+  eqb := String.eqb;
+  eqb_leibniz := String.eqb_eq
+}.
+
+Module Type Parser.
+  Import CharExtra.
+
+  Definition stream (A : Type) : Type := (list A * nat * nat).
+
+  Definition parser (A B : Type) `{HA : EqClass A} `{HB : EqClass B} : Type := 
+    (stream B) -> ((res A string) * list B * nat * nat).
+
+  (* parse: parser A ascii -> string -> res A string
+     * `parse p str`
+     * Runs the parser `p` over the string `str`.
+     *)
+  Definition parse {A : Type} `{HA : EqClass A} (p : (parser A ascii)) (str : string) : (res A string) :=
     match (p (String.list_ascii_of_string str , 1, 1)) with
     | (Ok x, _, _ , _) => Ok x
     | (Err msg, _, line, col) => 
         Err ("Error on line " ++ nat_to_string line ++ ", column " ++ nat_to_string col ++ ": " ++ msg)
+    end.
+
+  (* bind: parser A B -> (A -> parser C B) -> (stream B) -> parser C B
+    * `bind p funcp`
+    * Runs the parser `p` and upon success, applies `funcp` to the result and
+    * continue to parse.
+    *)
+  Definition bind {A B C : Type} `{EqClass A, EqClass B, EqClass C} 
+      (p : parser A B) (funcp : (A -> (parser C B))) : (parser C B) :=
+    fun (stream : stream B) =>
+      match (p stream) with
+      | (Ok x, cs', line', col') => funcp x (cs', line', col')
+      | (Err msg, cs', line', col') => ((Err msg), cs', line', col')
+      end.
+
+  (* bindResult: (A -> res B string) -> (parser A C) -> (parser B C)
+    * `bindResult func p`
+    * Runs the parser `p` and upon success, applies `func` to the result.
+    *)
+  Definition bindResult {A B C : Type} `{EqClass A, EqClass B, EqClass C}
+      (func : A -> res B string) (p : parser A C) : (parser B C) :=
+    fun (stream : (stream C)) =>
+      match p stream with
+      | (Ok x, cs', line', col') => (func x, cs', line', col')
+      | (Err err, cs', line', col') => (Err err, cs', line', col')
+      end.
+
+  (* map: (A -> B) -> parser A C -> parser B C
+    * `map func p`
+    * returns parser `p` and upon success, applies `func` to the result.
+    *)
+  Definition map {A B C : Type} `{EqClass A, EqClass B, EqClass C}
+      (func : A -> B) (p : parser A C) : (parser B C) :=
+    fun (stream : stream C) =>
+      match p stream with
+      | (Ok x, cs', line', col') =>
+          (Ok (func x), cs', line', col')
+      | (Err err, cs', line', col') =>
+          (Err err, cs', line', col')
+      end.
+
+  (* pure: 'a -> ('a, 'b) parser
+    * `pure x`
+    * A simple parser that successfully returns `x` without consuming any
+    * input.
+    *)
+  Definition pure {A B : Type} `{EqClass A, EqClass B}
+      (x : A) : (parser A B) :=
+    fun (stream : stream B) => 
+      match stream with
+      | (cs, line, col) => (Ok x, cs, line, col)
+      end.
+  
+  (* TODO: This is a type breaking thing! *)
+  (* fail: string -> parser A string
+    * `fail err`
+    * A simple parser that fails, returning `err`, without consuming any input.
+    *)
+  Definition fail {A : Type} `{EqClass A}
+      (err : string) : (parser A string) :=
+    fun (stream : stream _) =>
+      match stream with
+      | (cs, line, col) => (Err err, cs, line, col)
+      end.
+
+  (* eof: parser unit string
+    * `eof`
+    * A simple parser that succeeds exactly when there is no more input.
+    *)
+  Definition eof {A : Type} :=
+    fun (stream : stream string) =>
+      match stream with
+      | (cs, line, col) =>
+        match cs with
+        | nil => (Ok unit_val, cs, line, col)
+        | c::cs' => (Err "End of stream expected.", c::cs', line, col)
+        end
+      end.
+  
+  (* seq: parser A B -> parser C B -> parser C B
+    * `seq p1 p2`
+    * Runs parser `p1` and then, upon success, runs parser `p2`, discarding the
+    * previous results.
+    *)
+  Definition seq {A B C: Type} `{EqClass A, EqClass B, EqClass C}
+      (p1 : parser A B) (p2 : parser C B) : (parser C B) :=
+    fun (s : stream B) => 
+      bind p1 (fun _ => p2) s.
+
+  (* satisfy: (char -> bool) -> (char, char) parser
+    * `satisfy pred`
+    * A simple parser that succeeds exactly when `pred` returns true on the
+    * next element in the stream. Does not consume input upon failure.
+    *)
+  Example newline := "010"%char.
+  Definition satisfy (pred : ascii -> bool) : (parser ascii ascii) :=
+    fun (s : stream ascii) =>
+      match s with
+      | (cs, line, col) =>
+        match cs with
+        | nil => (Err "End of stream reached too early.", nil, line, col)
+        | c::cs' =>
+            if pred c
+            then if (c =? newline)%char
+                then (Ok c, cs', 1 + line, 1)
+                else (Ok c, cs', line, 1 + col)
+            else (Err "Failed to satisfy a predicate.", cs, line, col)
+        end
+      end.
+
+    (* label: string -> ('a, 'b) parser -> ('a, 'b) parser
+    * `label errMsg p`
+    * Runs parser `p` and if it fails without consuming input, then the error
+    * message is replaced by `errMsg`.
+    *)
+  Definition label {A B : Type} `{EqClass A, EqClass B}
+      (errMsg : string) (p : parser A B) : (parser A B) :=
+    fun (s : stream _) =>
+      match s with
+      | (cs, line, col) =>
+        match p (cs, line, col) with
+        | (Err str, cs', line', col') =>
+            if (andb (eqb line line') (andb (eqb col col') (eqb cs cs')))
+            then (Err errMsg, cs, line, col)
+            else (Err str, cs', line', col')
+        | (Ok x, cs', line', col') => (Ok x, cs', line', col')
+        end
+      end.
+
+  (* parser_return: 'a -> ('b, 'c) parser -> ('a, 'c) parser
+    * `parser_return x p`
+    * Runs parser `p` and if it succeeds replace the result with `x`.
+    *)
+  Definition parser_return {A B C : Type} `{EqClass A, EqClass B, EqClass C}
+      (x : A) (p : parser B C) : (parser A C) :=
+    fun (stream : stream _) =>
+      match p stream with
+      | (Ok _, cs', line', col') => (Ok x, cs', line', col')
+      | (Err err, cs', line', col') =>
+          (Err err, cs', line', col')
+      end.
+
+  (* char: char -> (char, char) parser
+    * `char c`
+    * Returns a simple parser that expects the next character in the stream to
+    * be `c`. Does not consume input upon failure.
+    *)
+  Definition char (inc : ascii) : (parser ascii ascii) :=
+    label ("Expected to see character '" ++ (String inc EmptyString) ++ "'.")
+        (satisfy (fun op => (eqb op inc)%char)).
+  
+  (* notChar: char -> (char, char) parser
+    * `notChar c`
+    * Returns a simple parser that expects the next character in the stream to
+    * not be `c`. Does not consume input upon failure.
+    *)
+  Definition notChar (inc : ascii) : (parser ascii ascii) :=
+    label ("Expected not to see character '" ++ (String inc EmptyString) ++ "'.")
+        (satisfy (fun op => (negb (eqb op inc)))).
+
+  (* oneOf: char list -> (char, char) parser
+    * `oneOf cs`
+    * A parser that succeeds exactly when the next character in the stream is
+    * one of the characters in the list `cs`. Does not consume input upon
+    * failure.
+    *)
+  Definition oneOf (incs : list ascii) : (parser ascii ascii) :=
+      label ("Expected one of the following characters """ ++ (String.string_of_list_ascii incs) ++ """.")
+          (satisfy (fun inc => if (List.in_dec (EqClass_impl_DecEq _) (inc) incs) then true else false)).
+
+  (* noneOf: char list -> (char, char) parser
+    * `noneOf cs`
+    * A parser that succeeds exactly when the next character in the stream is
+    * not one of the characters in the list `cs`. Does not consume input upon
+    * failure.
+    *)
+  Definition noneOf (incs : list ascii) : (parser ascii ascii) :=
+      label ("Expected not to see any of the following characters """ ++ (String.string_of_list_ascii incs) ++ """.")
+          (satisfy (fun inc => if (List.in_dec (EqClass_impl_DecEq _) inc incs) then false else true)).
+
+  (* anyChar: (char, char) parser
+    * A simple parser that succeeds so long as there is another character in
+    * the stream. Does not consume input upon failure.
+    *)
+  Definition anyChar := label "Expected any character." (satisfy (fun x => true)).
+
+  (* digit: (char, char) Parser
+    * A simple parser that succeeds upon seeing a digit, '0'..'9'. Does not
+    * consume input upon failure.
+    *)
+  Definition digit := label "Expected a digit." (satisfy CharExtra.isDigit).
+
+
+  (* octalDigit: (char, char) Parser
+    * A simple parser that succeeds upon seeing an octal numeral, '0'..'7'.
+    * Does not consume input upon failure.
+    *)
+  Definition octalDigit := 
+      label "Expected an octal digit." (satisfy CharExtra.isOctal).
+  (* hexDigit: (char, char) Parser
+    * A simple parser that succeeds upon seeing a hexadecimal numeral,
+    * '0'..'9' or 'a'..'f' or 'A'..'F'. Does not consume input upon
+    * failure.
+    *)
+  Definition hexDigit := 
+      label "Expected a hexidecimal digit." (satisfy CharExtra.isHex).
+  (* lower: (char, char) Parser
+    * A simple parser that succeeds upon seeing a lowercase ASCII
+    * character, 'a'..'z'. Does not consume input upon failure.
+    *)
+  Definition lower := 
+      label
+          "Expected a lower-case ascii character."
+          (satisfy CharExtra.isLower).
+  (* upper: (char, char) Parser
+    * A simple parser that succeeds upon seeing an uppercase ASCII
+    * character, 'A'..'Z'. Does not consume input upon failure.
+    *)
+  Definition upper := 
+      label
+          "Expected an upper-case ascii character."
+          (satisfy CharExtra.isUpper).
+  (* letter: (char, char) Parser
+    * A simple parser that succeeds upon seeing an ASCII alphabet
+    * character, 'a'..'z' or 'A'..'Z'. Does not consume input upon failure.
+    *)
+  Definition letter := 
+      label
+          "Expected an ascii alphabet character."
+          (satisfy CharExtra.isAlpha).
+  (* alphaNum: (char, char) Parser
+    * A simple parser that succeeds upon seeing an ASCII digit or alphabet
+    * character: 'a'..'z', 'A'..'Z', or '0'..'9'. Does not consume input
+    * upon failure.
+    *)
+  Definition alphaNum := 
+      label
+          "Expected an ascii alphanumeric character."
+          (satisfy CharExtra.isAlphaNum).
+  (* space: (char, char) Parser
+    * A simple parser that succeeds upon seeing any ASCII whitespace
+    * characters. Does not consume input upon failure.
+    *)
+  Definition space := 
+      label
+          "Expected an ascii whitespace character."
+          (satisfy CharExtra.isSpace).
+
+  (*
+    Helper for moving the lines and columns while parsing
+  *)
+  Fixpoint advancePos (cs' : list ascii) (lc : nat * nat) :=
+    let (line', col') := lc in
+    match cs' with
+    | nil => (line', col')
+    | c::cs'' => 
+        if (eqb c newline)
+        then advancePos cs'' (1 + line', 1) 
+        else advancePos cs'' (line', 1 + col')
+    end.
+
+  (*
+    Checks that the "exists l3, l1 ++ l3 = l2" essentially
+  *)
+  Fixpoint list_prefix {A : Type} `{EqClass A} (l1 l2 : list A) : bool :=
+    match l1, l2 with
+    | nil, _ => true
+    | h1 :: t1, h2 :: t2 => if (eqb h1 h2) then (list_prefix t1 t2) else false
+    | _, _ => false
+    end.
+
+  (* 
+    Drops the first 'n' elements of a list (if it goes off the end it just returns nill)
+  *)
+  Fixpoint list_drop {A : Type} `{EqClass A} (l : list A) (n : nat) : list A :=
+    match n with
+    | 0 => l
+    | S n' => 
+        match l with
+        | nil => nil (* TODO: Does this fit spec? *)
+        | h :: t => list_drop t n'
+        end
+    end.
+
+  (* string: string -> (string, char) parser
+  * `string str`
+  * A parser that succeeds when the characters of `str` are the characters
+  * that appear next in the stream. Does not consume input upon failure.
+  *)
+  Definition parser_string (str : string) : (parser string ascii) :=
+    fun (s : stream _) =>
+      match s with
+      | (cs, line, col) =>
+        let chars := String.list_ascii_of_string str in
+            if list_prefix chars cs
+            then
+                let (line', col') := advancePos chars (line, col)
+                in
+                    (Ok str, list_drop cs (String.length str), line', col')
+            else (Err ("Expect the literal string """ ++ str ++ """"),
+                    cs, line, col)
+      end.
+
+  Definition carriage_return : ascii := "013".
+
+  (* crlf: (char, char) parser
+    * A simple parser that succeeds upon seeing '\r\n' and returns '\n'. Does
+    * not consume input upon failure.
+    *)
+  Definition crlf :=
+      label "Expected a carriage return followed by a line feed."
+          (parser_return newline (parser_string (String carriage_return (String newline EmptyString)))).
+
+  (* choice: (('a, 'b) parser) list -> ('a, 'b) parser
+    * `choice ps`
+    * A parser that tries one parser after another until one succeeds or one
+    * fails and consumes input. Should the next parser to try fails and
+    * consumes input, then this function will do the same.
+    *)
+  Fixpoint choice {A B : Type} `{EqClass A, EqClass B} 
+      (ps : list (parser A B)) :=
+    fun stream =>
+      match stream with
+      | (cs, line, col) =>
+        match ps with
+        | nil => (Err "No more parsers to try", cs, line, col)
+        | p::ps' =>
+          match p (cs, line, col) with
+          | (Ok x, cs', line', col') =>
+              (Ok x, cs', line', col')
+          | (Err err, cs', line', col') =>
+              if (eqb line line') && (eqb col col') && (eqb cs cs')
+              then choice ps' (cs, line, col)
+              else (Err err, cs', line', col')
+          end
+      end
     end.
